New package init lemma, including functions and method sets

new/golang/defn/globals.v
@@ -1,5 +1,4 @@
 From New.golang.defn Require Export mem typing list.
-From New.golang.defn Require Import hex.
 
 Module globals.
 Section defns.
@@ -13,23 +12,32 @@ Definition unwrap : val :=
 
 Definition get (pkg_var_name : (go_string * go_string)): val :=
   λ: <>,
-    let: "varAddrs" := unwrap $ GlobalGet #("vars:" ++ pkg_var_name.1) in
+    let: (("varAddrs", "functions"), "typeToMethodSets") := unwrap $ GlobalGet #("pkg:" ++ pkg_var_name.1) in
     unwrap $ alist_lookup #(pkg_var_name.2) "varAddrs".
 
-Fixpoint alloc (vars : list (go_string * go_type)) : val :=
-  (λ: <>,
-    match vars with
-    | Datatypes.nil => #()
-    | (pair name t) :: vars =>
-        let: "addr" := ref_ty t (zero_val t) in
-        list.Cons (#name, "addr") (alloc vars)
-    end)%V.
+Fixpoint alloc_and_define
+  (pkg_name : go_string)
+  (vars : list (go_string * go_type))
+  (functions : list (go_string * val))
+  (msets : list (go_string * (list (go_string * val)))) : val :=
+  let functions_val := alist_val functions in
+  let msets_val := alist_val ((λ '(name, mset), (name, alist_val mset)) <$> msets) in
+  λ: <>,
+    GlobalPut #pkg_name ((fix alloc (vars : list (go_string * go_type)) : expr :=
+        (match vars with
+         | Datatypes.nil => list.Nil
+         | (pair name t) :: vars =>
+             let: "addr" := ref_ty t (zero_val t) in
+             list.Cons (#name, "addr") (alloc vars)
+         end)%E) vars, functions_val, msets_val)
+.
 
-Definition package_init (pkg_name : go_string) (vars : list (go_string * go_type)) : val :=
+Definition package_init (pkg_name : go_string) vars functions msets : val :=
   λ: "init",
     match: GlobalGet #("pkg:" ++ pkg_name) with
       SOME <> => #()
-    | NONE => alloc vars #() ;; "init" #() ;; GlobalPut #("pkg:" ++ pkg_name) #()
+    | NONE => alloc_and_define pkg_name vars functions msets #() ;;
+             "init" #()
     end.
 
 End defns.
@@ -40,7 +48,7 @@ Context `{ffi_syntax}.
 
 Definition func_call (pkg_func_name : go_string * go_string) : val :=
   λ: <>,
-    let: "functions" := globals.unwrap $ GlobalGet #("funcs:" ++ pkg_func_name.1) in
+    let: (("varAddrs", "functions"), "typeToMethodSets") := globals.unwrap $ GlobalGet #("pkg:" ++ pkg_func_name.1) in
     globals.unwrap $ alist_lookup #(pkg_func_name.2) "functions".
 
 Definition method_call (pkg_type_method_name : go_string * go_string * go_string) : val :=
@@ -48,7 +56,7 @@ Definition method_call (pkg_type_method_name : go_string * go_string * go_string
     let pkg_name := pkg_type_method_name.1.1 in
     let type_name := pkg_type_method_name.1.2 in
     let method_name := pkg_type_method_name.2 in
-    let: "typeToMethodSet" := globals.unwrap $ GlobalGet #("type:" ++ pkg_name) in
+    let: (("varAddrs", "functions"), "typeToMethodSets") := globals.unwrap $ GlobalGet #("pkg:" ++ pkg_name) in
     let: "methodSet" := globals.unwrap $ GlobalGet #("type:" ++ type_name) in
     globals.unwrap $ alist_lookup #method_name "methodSet".
 
