new/golang/defn/interface.v
@@ -1,6 +1,5 @@
 From Perennial.goose_lang Require Import notation.
 From New.golang.defn Require Import struct typing globals.
-From New.golang.defn Require Import hex.
 
 Module interface.
 Section goose_lang.
